Impl/StateModel.i.dfy
@@ -256,17 +256,19 @@ module StateModel {
   // Functional model of the DiskIOHandler
 
   datatype IO =
-    | IOInit(id: uint64)
+    | IOInit(id: uint64, id2: uint64)
     | IOReqRead(id: uint64, reqRead: D.ReqRead)
     | IOReqWrite(id: uint64, reqWrite: D.ReqWrite)
+    | IOReqWrite2(id: uint64, id2: uint64, reqWrite1: D.ReqWrite, reqWrite2: D.ReqWrite)
     | IORespRead(id: uint64, respRead: D.RespRead)
     | IORespWrite(id: uint64, respWrite: D.RespWrite)
 
   function diskOp(io: IO) : D.DiskOp {
     match io {
-      case IOInit(id) => D.NoDiskOp
+      case IOInit(id, id2) => D.NoDiskOp
       case IOReqRead(id, reqRead) => D.ReqReadOp(id, reqRead)
       case IOReqWrite(id, reqWrite) => D.ReqWriteOp(id, reqWrite)
+      case IOReqWrite2(id1, id2, reqWrite1, reqWrite2) => D.ReqWrite2Op(id1, id2, reqWrite1, reqWrite2)
       case IORespRead(id, respRead) => D.RespReadOp(id, respRead)
       case IORespWrite(id, respWrite) => D.RespWriteOp(id, respWrite)
     }
